end of day 31/07/19

inference-tool/src/main/scala/inference/Dirties.scala
@@ -16,7 +16,7 @@ object Dirties {
     case VName.R(n) => s"r${Code_Numeral.integer_of_nat(n)}"
   }
 
-  def toZ3(a: AExp.aexp): String =  a match {
+  def toZ3(a: AExp.aexp): String = a match {
     case AExp.L(Value.Numa(n)) => Code_Numeral.integer_of_int(n).toString
     case AExp.L(Value.Str(s)) => "\"" + s + "\""
     case AExp.V(v) => s"${toZ3(v)}Value"
@@ -24,13 +24,13 @@ object Dirties {
     case AExp.Minus(a1, a2) => s"(- (${toZ3(a1)}) (${toZ3(a2)}))"
   }
 
-  def toZ3(a: Type_Inference.typea): String = a match  {
+  def toZ3(a: Type_Inference.typea): String = a match {
     case Type_Inference.NUM() => "Int"
     case Type_Inference.STRING() => "String"
     case Type_Inference.UNBOUND() => "String"
   }
 
-  def toZ3(g: GExp.gexp, types: Map[VName.vname, Type_Inference.typea]): String =  g match {
+  def toZ3(g: GExp.gexp, types: Map[VName.vname, Type_Inference.typea]): String = g match {
     case GExp.Bc(a) => a.toString()
     case GExp.Eq(a1, a2) => s"(= ${toZ3(a1)} ${toZ3(a2)})"
     case GExp.Gt(a1, a2) => s"(> ${toZ3(a1)} ${toZ3(a2)})"
@@ -45,18 +45,16 @@ object Dirties {
   def satisfiable(g: GExp.gexp): Boolean = {
     if (sat_memo isDefinedAt g) {
       return sat_memo(g)
-    }
-    else {
+    } else {
       val maybe_types = Type_Inference.infer_types(g)
       maybe_types match {
         case None => false
         case Some(types) => {
           var z3String = s"(declare-datatype Option (par (X) ((none) (some (val X)))))\n" +
-          types.map(t => t match {
+            types.map(t => t match {
               case (k, v) => s"(declare-const ${toZ3(k)} (Option ${toZ3(v)}))\n(declare-const ${toZ3(k)}Value (${toZ3(v)}))"
-            }
-          ).foldLeft("")(((x, y) => x + y + "\n"))+
-          s"(assert ${toZ3(g, types)})\n(check-sat)"
+            }).foldLeft("")(((x, y) => x + y + "\n")) +
+            s"(assert ${toZ3(g, types)})\n(check-sat)"
 
           // Log.root.debug(g.toString)
           // Log.root.debug(z3String)
@@ -87,12 +85,11 @@ object Dirties {
 
   def randomMember[A](f: FSet.fset[A]): Option[A] = f match {
     case FSet.fset_of_list(l) =>
-        if (l == List()) {
-          None
-        }
-        else {
-          Some(Random.shuffle(l).head)
-        }
+      if (l == List()) {
+        None
+      } else {
+        Some(Random.shuffle(l).head)
+      }
   }
 
   def addLTL(f: String, e: String) = {
@@ -105,95 +102,82 @@ object Dirties {
     pw.close()
   }
 
-  def alwaysDifferentOutputsDirectSubsumption[A](m1: IEFSM,
-                                              m2: IEFSM,
-                                              s:Nat.nat,
-                                              s_prime: Nat.nat,
-                                              t1: Transition.transition_ext[A],
-                                              t2: Transition.transition_ext[A]):Boolean = {
-      // This is a stub but should be safe enough
-      true
+  // We're checking for the existence of a trace that gets us to the right
+  // states in the respective machines such that we can take t2 so we check
+  // the global negation of this to see if there's a counterexample
+  def alwaysDifferentOutputsDirectSubsumption[A](
+    e1: IEFSM,
+    e2: IEFSM,
+    s1: Nat.nat,
+    s2: Nat.nat,
+    t2: Transition.transition_ext[A]): Boolean = {
+    val f = "intermediate_" + System.currentTimeMillis()
+    TypeConversion.doubleEFSMToSALTranslator(Inference.tm(e1), "e1", Inference.tm(e2), "e2", f)
+    addLTL(s"salfiles/${f}.sal", s"composition: MODULE = (RENAME O TO O_e1 IN e1) || (RENAME O TO O_e2 IN e2);\n" +
+      s"canTake: THEOREM composition |- G(cfstate.1 = ${TypeConversion.salState(s1)} AND cfstate.2 = ${TypeConversion.salState(s2)} => NOT(input_sequence ! size?(I) = ${Code_Numeral.integer_of_nat(Transition.Arity(t2))} AND ${efsm2sal.guards2sal(Transition.Guard(t2))}));")
+    val output = Seq("bash", "-c", s"cd salfiles; sal-smc --assertion='${f}{100}!canTake'").!!
+    if (!output.toString.startsWith("Counterexample")) {
+      println(s"G(cfstate.1 = ${TypeConversion.salState(s1)} AND cfstate.2 = ${TypeConversion.salState(s2)} => NOT(input_sequence ! size?(I) = ${Code_Numeral.integer_of_nat(Transition.Arity(t2))} AND ${efsm2sal.guards2sal(Transition.Guard(t2))}));")
+      println(s"sal-smc --assertion='${f}{100}!canTake'")
+    }
+    return (output.toString.startsWith("Counterexample"))
   }
 
   def initiallyUndefinedContextCheck(e: IEFSM, r: Nat.nat, s: Nat.nat): Boolean = {
-    val f = "intermediate_"+System.currentTimeMillis()
+    println("initiallyUndefinedContextCheck")
+    val f = "intermediate_" + System.currentTimeMillis()
     TypeConversion.efsmToSALTranslator(Inference.tm(e), f)
 
     addLTL("salfiles/" + f + ".sal", s"  initiallyUndefined: THEOREM MichaelsEFSM |- G(cfstate = State_${Code_Numeral.integer_of_nat(s)} => r_${Code_Numeral.integer_of_nat(r)} = value_option ! None);")
 
-    val output = Seq("bash", "-c", "cd salfiles; sal-smc --assertion='" + f + "{100}!initiallyUndefined'").!!
+    val output = Seq("bash", "-c", s"cd salfiles; sal-smc --assertion='${f}{100}!initiallyUndefined'").!!
     if (output.toString != "proved.\n") {
       print(output)
     }
     return (output.toString == "proved.\n")
   }
 
-  def salValue(v: Value.value): String = v match {
-    case Value.Str(s) => s"STR(String_$s)"
-    case Value.Numa(n) => s"NUM(${Code_Numeral.integer_of_int(n)})"
-  }
-
-  def generaliseOutputContextCheck(l: String, ePrime: IEFSM, e: IEFSM, r: Nat.nat, v: Value.value, s_old: Nat.nat, s_new: Nat.nat): Boolean = {
-    val f_old = "orig_"+System.currentTimeMillis()
-    TypeConversion.efsmToSALTranslator(Inference.tm(e), f_old)
-    val inxLabel = Code_Generation.input_updates_register(ePrime)
-    addLTL("salfiles/" + f_old + s".sal", s"  inputValue: THEOREM MichaelsEFSM |-\n" +
-      s"    U(cfstate /= NULL_STATE, cfstate=State_${Code_Numeral.integer_of_nat(s_old)}) =>\n"+
-      s"    U(label = ${inxLabel._2} => I(1) = ${salValue(v)}, X(cfstate = NULL_STATE));")
-
-    val f_new = "intermediate_"+System.currentTimeMillis()
-    TypeConversion.efsmToSALTranslator(Inference.tm(ePrime), f_new)
-    addLTL("salfiles/" + f_new + ".sal", s"  generaliseOutput: THEOREM MichaelsEFSM |-\n"+
-      s"    U(cfstate /= NULL_STATE, cfstate = State_${Code_Numeral.integer_of_nat(s_new)}) =>\n"+
-      s"    U(label = select => I(${Code_Numeral.integer_of_nat(inxLabel._1)+1}) = ${salValue(v)}, cfstate = NULL_STATE) =>\n"+
-      s"    U(cfstate = State_${Code_Numeral.integer_of_nat(s_new)} => r_1 = Some(${salValue(v)}), cfstate=NULL_STATE);")
-
-
-    println(s"sal-smc --assertion='${f_old}{100}!inputValue'")
-    val output1 = Seq("bash", "-c", s"cd salfiles; sal-smc --assertion='${f_old}{100}!inputValue'").!!
-    println(output1)
-
-    println(s"sal-smc --assertion='${f_new}{100}!generaliseOutput'")
-    val output2 = Seq("bash", "-c", s"cd salfiles; sal-smc --assertion='${f_new}{100}!generaliseOutput'").!!
-    println(output2)
-
-    return (output1.toString == "proved.\n" && output2.toString == "proved.\n")
-  }
-
-  def canTake(e: Types.IEFSM, s: Nat.nat, t: Types.Transition): Boolean = {
-    val f = "intermediate_"+System.currentTimeMillis()
-    TypeConversion.efsmToSALTranslator(Inference.tm(e), f)
-
-    addLTL("salfiles/" + f + ".sal", s"  canTake: THEOREM MichaelsEFSM |- G(cfstate = State_${Code_Numeral.integer_of_nat(s)} => EXISTS (I : input_sequence ! Sequence): (${efsm2sal.guards2sal(Transition.Guard(t))}));")
-
-    val output = Seq("bash", "-c", "cd salfiles; sal-smc --assertion='" + f + "{100}!canTake'").!!
+  def generaliseOutputContextCheck(v: Value.value, r: Nat.nat, s1: Nat.nat, s2: Nat.nat, e1: IEFSM, e2: IEFSM): Boolean = {
+    val f = "intermediate_" + System.currentTimeMillis()
+    TypeConversion.doubleEFSMToSALTranslator(Inference.tm(e1), "e1", Inference.tm(e2), "e2", f)
+    addLTL(s"salfiles/${f}.sal", s"composition: MODULE = (RENAME O TO O_e1 IN e1) || (RENAME O TO O_e2 IN e2);\n" +
+      s"checkRegValue: THEOREM composition |- G(cfstate.1 = ${TypeConversion.salState(s1)} AND cfstate.2 = ${TypeConversion.salState(s2)} => r_${Code_Numeral.integer_of_nat(r)}.2 = Some(${TypeConversion.salValue(v)}));")
+    val output = Seq("bash", "-c", s"cd salfiles; sal-smc --assertion='${f}{100}!checkRegValue'").!!
     if (output.toString != "proved.\n") {
       print(output)
     }
     return (output.toString == "proved.\n")
   }
 
+  // Here we check to see if globally we can never be in both states
+  // If there's a counterexample then there exists a trace which gets us to
+  // both states
   def acceptsAndGetsUsToBoth(a: IEFSM,
-                            b: IEFSM,
-                            s: Nat.nat,
-                            s_prime: Nat.nat): Boolean = {
-                              true
-                            }
+    b: IEFSM,
+    s1: Nat.nat,
+    s2: Nat.nat): Boolean = {
+    val f = "intermediate_" + System.currentTimeMillis()
+    TypeConversion.doubleEFSMToSALTranslator(Inference.tm(a), "e1", Inference.tm(b), "e2", f)
+    addLTL(s"salfiles/${f}.sal", s"composition: MODULE = (RENAME O TO O_e1 IN e1) || (RENAME O TO O_e2 IN e2);\n" +
+      s"getsUsToBoth: THEOREM composition |- G(NOT(cfstate.1 = ${TypeConversion.salState(s1)} AND cfstate.2 = ${TypeConversion.salState(s2)}));")
+    val output = Seq("bash", "-c", s"cd salfiles; sal-smc --assertion='${f}{100}!getsUsToBoth'").!!
+    return (output.toString.startsWith("Counterexample"))
+  }
 
   def scalaDirectlySubsumes(a: IEFSM,
-                            b: IEFSM,
-                            s: Nat.nat,
-                            s_prime: Nat.nat,
-                            t1: Transition.transition_ext[Unit],
-                            t2: Transition.transition_ext[Unit]): Boolean = {
-                              if (Store_Reuse_Subsumption.generalise_output_direct_subsumption(t2, t1, b, a, s, s_prime)) {
-                                // println("n")
-                                return false
-                              }
-                              // else {
-                                println(s"Does ${PrettyPrinter.transitionToString(t1)} directly subsume ${PrettyPrinter.transitionToString(t2)}? (y/N)")
-                                val subsumes = readLine("") == "y"
-                                subsumes
-                              // }
-                            }
+    b: IEFSM,
+    s: Nat.nat,
+    s_prime: Nat.nat,
+    t1: Transition.transition_ext[Unit],
+    t2: Transition.transition_ext[Unit]): Boolean = {
+    if (Store_Reuse_Subsumption.generalise_output_direct_subsumption(t2, t1, b, a, s, s_prime)) {
+      // println("n")
+      return false
+    }
+    // else {
+    println(s"Does ${PrettyPrinter.transitionToString(t1)} directly subsume ${PrettyPrinter.transitionToString(t2)}? (y/N)")
+    val subsumes = readLine("") == "y"
+    subsumes
+    // }
   }
+}
